platform/cito/LinkSpecFacts.v
@@ -14,67 +14,77 @@ Module Make (Import E : ADT).
     Notation FName := SyntaxFunc.Name.
     Notation MName := GoodModule.Name.
 
-    Definition imports_exports_mapsto lbl spec modules imports :=
-      (exists ispec m f,
-         spec = Internal ispec /\
-         List.In m modules /\
-         List.In f (Functions m) /\
-         ispec = f /\ 
-         lbl = (MName m, FName f)) \/
-      (exists fspec,
-         spec = Foreign fspec /\
-         find lbl imports = Some fspec).
-
-    Definition imports_exports_in lbl modules (imports : t ForeignFuncSpec) :=
-      (exists m f,
-         List.In m modules /\
-         List.In f (Functions m) /\
-         lbl = (MName m, FName f)) \/
-      In lbl imports.
-
     Require Import GeneralTactics.
 
-    Lemma imports_exports_mapsto_in : forall modules imports lbl spec, imports_exports_mapsto lbl spec modules imports -> imports_exports_in lbl modules imports.
-      unfold imports_exports_mapsto, imports_exports_in.
+    Lemma label_mapsto_in : forall modules imports lbl spec, label_mapsto modules imports lbl spec -> label_in modules imports lbl.
+      unfold label_mapsto, label_in.
       intros.
       openhyp.
       left; descend; eauto.
       right; eapply MapsTo_In; eapply find_mapsto_iff; eauto.
     Qed.
 
-    Definition specs_equal specs modules imports := forall lbl spec, find lbl specs = Some spec <-> imports_exports_mapsto lbl spec modules imports.
+    Lemma label_in_mapsto : forall modules imports lbl, label_in modules imports lbl -> exists spec, label_mapsto modules imports lbl spec.
+      unfold label_mapsto, label_in.
+      intros.
+      openhyp.
+      subst; simpl in *.
+      descend; left; descend; eauto.
+      eapply In_MapsTo in H; openhyp.
+      eapply find_mapsto_iff in H.
+      descend; right; descend; eauto.
+    Qed.
 
-    Lemma specs_equal_agree : forall specs modules imports, specs_equal specs modules imports -> forall stn fs, stn_good_to_use modules imports stn -> fs_good_to_use modules imports fs stn -> specs_env_agree specs (from_bedrock_label_map (Labels stn), fs stn).
+    Definition specs_equal specs modules imports := forall lbl spec, find lbl specs = Some spec <-> label_mapsto modules imports lbl spec.
+
+    Lemma specs_equal_in : forall specs modules imports, specs_equal specs modules imports -> forall lbl, In lbl specs <-> label_in modules imports lbl.
+      split; intros.
+      eapply In_MapsTo in H0.
+      openhyp.
+      eapply label_mapsto_in.
+      eapply H.
+      eapply find_mapsto_iff; eauto.
+      eapply label_in_mapsto in H0; openhyp.
+      eapply MapsTo_In.
+      eapply find_mapsto_iff.
+      eapply H; eauto.
+    Qed.
+
+    Lemma specs_equal_agree : forall specs modules imports, specs_equal specs modules imports -> forall stn fs, env_good_to_use modules imports stn fs -> specs_env_agree specs (from_bedrock_label_map (Labels stn), fs stn).
       intros.
       split.
 
       unfold labels_in_scope.
       intros.
       unfold from_bedrock_label_map in *; simpl in *.
-      eapply In_MapsTo in H2.
-      openhyp.
-      eapply H0.
-      eapply imports_exports_mapsto_in.
-      eapply H.
-      eapply find_mapsto_iff; eauto.
+      eapply H0; eapply specs_equal_in; eauto.
 
+      split.
+      Focus 2.
       unfold specs_fs_agree.
       unfold from_bedrock_label_map in *; simpl in *.
       split; intros.
 
-      eapply H1 in H2.
-      destruct H2.
-      destruct H2.
+      eapply H0 in H1.
+      destruct H1.
+      destruct H1.
       descend.
       eauto.
       eapply H; eauto.
 
       openhyp.
-      eapply H1.
+      eapply H0.
       eexists.
       split.
       eauto.
       eapply H; eauto.
+
+      unfold specs_stn_injective.
+      intros.
+      unfold from_bedrock_label_map in *; simpl in *.
+      eapply H0; eauto.
+      eapply specs_equal_in; eauto.
+      eapply specs_equal_in; eauto.
     Qed.
 
   End TopSection.
