platform/cito/GeneralTactics3.v
@@ -6,3 +6,8 @@ Ltac unfold_all :=
 Ltac inv_clear H := 
   inversion H; unfold_all; subst; clear H.
 
+Ltac eapply_in_any t :=
+  match goal with
+      H : _ |- _ => eapply t in H
+  end.
+    
